vstd development

VerusLean/Vstd/Map/Defs.lean
@@ -6,76 +6,156 @@ namespace Vstd
   Verus `Vstd` maps.
 -/
 class VMapLikeF (M : Type u → Type v → Type w)
+  (S_key : outParam (Type u → Type x)) [VSetLikeF S_key]
+  (S_val : outParam (Type v → Type y)) [VSetLikeF S_val]
   where
   empty : M α β
-  keys : M α β → Set α
-  values : M α β → Set β
-  memKeys : M α β → α → Prop :=
+  -- do we want an infinite map type class?
+  total : (α → β) → M α β
+  new : (α → Bool) → (α → β) → M α β
+  -- keys : M α β → Set α
+  -- values : M α β → Set β
+  keys : M α β → S_key α
+  values : M α β → S_val β
+  memKeys [DecidableEq α] : M α β → α → Prop :=
     fun m k => k ∈ keys m
   memValues : M α β → β → Prop :=
     fun m v => v ∈ values m
-  get? : M α β → α → Option β
-  get : (m : M α β) → (k : α) → (h : memKeys m k) → β
-  get! {α : Type u} {β : Type v} [Inhabited β] : (m : M α β) → (k : α) → β
+  -- CZ: how does implementation guarantee this is decidable?
+  -- memKeys [DecidableEq α] [Decidable (k ∈ keys m)] : M α β → α → Bool
+    -- := fun m k => decide (k ∈ keys m)
+  -- memValues : M α β → β → Bool
+  get? [DecidableEq α] : M α β → α → Option β
+  get [DecidableEq α] [Inhabited β] : (m : M α β) → (k : α) → (h : memKeys m k) → β
+  get! [DecidableEq α] [Inhabited β] : (m : M α β) → (k : α) → β
   insert : (m : M α β) → (k : α) → (v : β) → M α β
   remove : (m : M α β) → (k : α) → M α β
-  union_prefer_right : (m₁ m₂ : M α β) → M α β
-  union_prefer_left : (m₁ m₂ : M α β) → M α β :=
+  removeKeys : (m : M α β) → (ks : Set α) → M α β
+  restrict : (m : M α β) → (ks : Set α) → M α β
+  isEqualOnKey [DecidableEq α] [DecidableEq β] : (m₁ m₂ : M α β) → (k : α) → Bool
+  agrees [DecidableEq α] [DecidableEq β] : (m₁ m₂ : M α β) → Bool
+  size : M α β → Nat
+  submapOf {α : Type u} {β : Type v} [DecidableEq α] [DecidableEq β]: M α β → M α β → Bool
+  union_prefer_right [DecidableEq α] : (m₁ m₂ : M α β) → M α β
+  union_prefer_left [DecidableEq α] : (m₁ m₂ : M α β) → M α β :=
     fun m₁ m₂ => union_prefer_right m₂ m₁
+  mapEntires : (m : M α β) → (f : α → β → γ) → M α γ
   mapValues : (m : M α β) → (f : β → γ) → M α γ
+  isInjective : (m : M α β) → Bool
   ofList : List (α × β) → M α β :=
     fun l => l.foldl (fun m p => insert m p.1 p.2) empty
 
 namespace VMapLikeF
 
-variable {M : Type u → Type v → Type w} [VMapLikeF M] {α : Type u} {β : Type v}
+-- variable {M : Type u → Type v → Type w} [VMapLikeF M] {α : Type u} {β : Type v}
+variable {M : Type u → Type v → Type w} {S_key : Type u → Type w_key} [VSetLikeF S_key]
+  {S_val : Type v → Type w_val} [VSetLikeF S_val] [VMapLikeF M S_key S_val] {α : Type u} {β : Type v}
 
-abbrev domain (m : M α β) : Set α := keys m
-abbrev range (m : M α β) : Set β := values m
-abbrev codomain (m : M α β) : Set β := values m
+abbrev domain (m : M α β) : S_key α := keys m
+abbrev range (m : M α β) : S_val β := values m
+abbrev codomain (m : M α β) : S_val β := values m
 
 instance instEmptyCollection : EmptyCollection (M α β) := ⟨empty⟩
 instance instInhabited : Inhabited (M α β) := ⟨empty⟩
 instance instSingleton : Singleton (α × β) (M α β) := ⟨fun p => insert ∅ p.1 p.2⟩
 instance instInsert : Insert (α × β) (M α β) := ⟨fun p m => insert m p.1 p.2⟩
-instance instMembershipKeys : Membership α (M α β) := ⟨memKeys⟩
-instance instMembershipValues : Membership β (M α β) := ⟨memValues⟩
-instance instMembership : Membership (α × β) (M α β) := ⟨fun m p => p.1 ∈ m ∧ p.2 ∈ m⟩
-instance instUnion : Union (M α β) := ⟨union_prefer_right⟩
+instance instMembershipKeys [DecidableEq α] : Membership α (M α β) := ⟨fun m k => memKeys m k = true⟩
+instance instMembershipValues : Membership β (M α β) := ⟨fun m v => memValues m v = true⟩
+instance instMembership [DecidableEq α] [Inhabited β] : Membership (α × β) (M α β) := ⟨fun m p => p.1 ∈ keys m ∧ p.2 ∈ values m ∧ get! m p.1 = p.2⟩
+instance instUnion [DecidableEq α] : Union (M α β) := ⟨union_prefer_right⟩
 instance instCoeOfList : Coe (List (α × β)) (M α β) := ⟨ofList⟩
-instance instGetElem : GetElem (M α β) α β (fun m k => memKeys m k) := ⟨get⟩
-instance instGetElem? : GetElem? (M α β) α β (fun m k => memKeys m k) where
+instance instGetElem [DecidableEq α] [Inhabited β] : GetElem (M α β) α β (fun m k => memKeys m k) := ⟨get⟩
+instance instGetElem? [DecidableEq α] [Inhabited β] : GetElem? (M α β) α β (fun m k => memKeys m k) where
   getElem? := get?
   getElem! := get!
 
 end VMapLikeF /- namespace -/
 
-class LawfulVMapLikeF (M : Type u → Type v → Type w)
+class LawfulVMapLikeF
+  (M : Type u₁ → Type v₁ → Type w₁)
+  (S_key : outParam (Type u₁ → Type w_key)) [VSetLikeF S_key] [LawfulVSetLikeF S_key]
+  (S_val : outParam (Type v₁ → Type w_val)) [VSetLikeF S_val] [LawfulVSetLikeF S_val]
   extends
-    VMapLikeF M
+    VMapLikeF M S_key S_val
   where
-  protected ext (m₁ m₂ : M α β) : (∀ (k : α), k ∈ keys m₁ ↔ k ∈ keys m₂) → (∀ (k : α), get? m₁ k = get? m₂ k) → m₁ = m₂
+  protected ext [DecidableEq α] (m₁ m₂ : M α β) : (∀ (k : α), k ∈ keys m₁ ↔ k ∈ keys m₂ ∧ get? m₁ k = get? m₂ k) → m₁ = m₂
   keys_empty : keys (∅ : M α β) = ∅
   values_empty : values (∅ : M α β) = ∅
-  memKeys_iff : ∀ (m : M α β) (k : α), memKeys m k ↔ k ∈ keys m
+  memKeys_iff [DecidableEq α] : ∀ (m : M α β) (k : α), memKeys m k ↔ k ∈ keys m
   memValues_iff : ∀ (m : M α β) (v : β), memValues m v ↔ v ∈ values m
-  mem_insert_iff {k k' : α} {v v' : β} {m : M α β}
-      : (k', v') ∈ (insert m k v) ↔ (k = k' ∧ v = v') ∨ (k', v') ∈ m
+  mem_insert_iff {α β} [DecidableEq α] [Inhabited β] {k₁ k₂ : α} {v₁ v₂ : β} {m : M α β} :
+    (k₂, v₂) ∈ (insert m k₁ v₁) ↔ (k₁ = k₂ ∧ v₁ = v₂) ∨ (k₂, v₂) ∈ m
+  memKeys_insert_iff {α β} {k₁ k₂ : α} {v₁ v₂ : β} {m : M α β} :
+    k₂ ∈ keys (insert m k₁ v₁) ↔ k₂ = k₁ ∨ k₂ ∈ keys m
+  mem_remove_iff {α β} [DecidableEq α] [Inhabited β] {k₁ k₂ : α} {v : β} {m : M α β} :
+    (k₂, v) ∈ (remove m k₁) ↔ k₂ ≠ k₁ ∧ (k₂, v) ∈ m
+  memKeys_remove_iff {α β} [DecidableEq α] {k₁ k₂ : α} {m : M α β} :
+    k₂ ∈ keys (remove m k₁) ↔ k₂ ≠ k₁ ∧ k₂ ∈ keys m
+
+  get?_insert [DecidableEq α] (k₁ k₂ : α) (v : β) (m : M α β) :
+    get? (insert m k₁ v) k₂ = if k₁ = k₂ then some v else get? m k₂
+  get?_remove [DecidableEq α] (k₁ k₂ : α) (m : M α β) :
+    get? (remove m k₁) k₂ = if k₁ = k₂ then none else get? m k₂
+
+  memKeys_insert {α β} [DecidableEq α] (k : α) (v : β) (m : M α β) :
+    memKeys (insert m k v) k
 
 open LawfulVMapLikeF in
 attribute [simp] keys_empty values_empty
-attribute [ext] LawfulVMapLikeF.ext
+-- attribute [ext] LawfulVMapLikeF.ext
 
-class VMapF (M : Type u → Type v → Type w)
-  extends
-    VMapLikeF M
+-- class VMapF (M : Type u → Type v → Type w)
+--   extends
+--     VMapLikeF M
 
-class VMap (M : Type u → Type v → Type w) (α : Type u) (β : Type v)
-  extends VMapLikeF M
+-- class VMap (M : Type u → Type v → Type w) (α : Type u) (β : Type v)
+--   extends VMapLikeF M
 
-class LawfulVMap (M : Type u → Type v → Type w) (α : Type u) (β : Type v)
-  extends
-    LawfulVMapLikeF M,
-    LawfulGetElem (M α β) α β (fun m k => memKeys m k)
+-- class LawfulVMap (M : Type u → Type v → Type w) (α : Type u) (β : Type v)
+--   extends
+--     LawfulVMapLikeF M,
+--     LawfulGetElem (M α β) α β (fun m k => memKeys m k)
+--   where
+
+open Std in
+def MapVstdTranslationNames : HashMap Lean.Name Lean.Name := HashMap.ofList <|
+  List.map (f := fun ⟨x, y⟩ => (String.toName s!"Vstd.Map.{x}", String.toName y)) <| [
+  /- from current map.rs -/
+  ("empty", "VMapLikeF.empty"),
+  -- There is a discussion about set.mk_map: https://github.com/verus-lang/verus/discussions/1666
+  ("total", "VMapLikeF.total"), -- do we want an infinite map type class?
+  ("new", "VMapLikeF.new"),
+  ("dom", "VMapLikeF.domain"),
+   /- Verus: For keys not in the domain, the result is meaningless and arbitrary.
+      But Lean will panic if key not in domain.
+      `get` and `get?` don't have the same signature as `index`. -/
+  ("index", "VMapLikeF.get!"),
+  ("spec_index", "VMapLikeF.get!"), -- same as index
+  ("insert", "VMapLikeF.insert"),
+  ("remove", "VMapLikeF.remove"),
+  ("len", "VMapLikeF.size"), -- or LawfulVMapLikeF.size?
+
+  /- from current map_lib.rs -/
+  ("is_full", "VMapLikeF.keys |> VSetInfF.full"), -- need something beyond a translation table to operate on the domain set
+  ("is_empty", "VMapLikeF.keys |> VSetLikeF.empty"), -- same
+  ("contains_key", "VMapLikeF.memKeys"),
+  ("contains_value", "VMapLikeF.memValues"),
+  ("index_opt", "VMapLikeF.get?"),
+  ("values", "VMapLikeF.values"),
+  ("contains_pair", "VMapLikeF.instMembership"), -- not sure
+  ("submap_of", "VMapLikeF.submapOf"),
+  ("spec_le", "VMapLikeF.submapOf"), -- same as submap_of
+  ("union_prefer_right", "VMapLikeF.union_prefer_right"),
+  ("remove_keys", "VMapLikeF.removeKeys"),
+  ("restrict", "VMapLikeF.restrict"),
+  ("is_equal_on_key", "VMapLikeF.isEqualOnKey"),
+  ("agrees", "VMapLikeF.agrees"),
+  ("map_entires", "VMapLikeF.mapEntries"),
+  ("map_values", "VMapLikeF.mapValues"),
+  ("is_injective", "VMapLikeF.isInjective"),
+  ("invert", ""), -- ignored for now, as it requires a different type class
+
+  -- Missing entries for `is_monotonic` and `is_monotonic_from` under `impl Map<int, int>`
+]
 
 end Vstd
