VerusLean/Vstd/Set/Defs.lean
@@ -1,3 +1,4 @@
+import VerusLean.Vstd.Seq
 import Std.Data.HashMap
 
 namespace Vstd
@@ -10,14 +11,18 @@ class VSetLikeF (S : Type u → Type v)
     Functor S
   where
   mem : {α : Type u} → S α → α → Prop
-  empty : {α : Type u} → S α
+  -- mem : {α : Type u} → S α → α → Bool -- if [DecidableEq α] here then Shim.lean can be Cedar's defn, but then not sure how to satisfy `instance instMembership`
+  empty : {α : Type u} → S α -- why is the empty set an infinite set in Verus?
   insert : {α : Type u} → α → S α → S α
-  remove : {α : Type u} → α → (S α) → (S α)
+  remove : {α : Type u} → α → S α → S α
   singleton : {α : Type u} → α → S α :=
     fun a => insert a empty
   -- To get around `noncomputable instance` for `Shim.lean`, we enforce that `α` be inhabited.
-  choose {α : Type u} [Inhabited α] : (s : S α) → (h : ∃ x, mem s x) → α
-  subset : {α : Type u} → S α → S α → Prop :=
+  -- choose {α : Type u} [Inhabited α] : (s : S α) → (h : ∃ x, mem s x) → α
+  /- CZ: How about that we don't require (h : ∃ x, mem s x), and just say we
+     don't care what ∅.choose returns, as long as α is inhabited it's fine -/
+  choose {α : Type u} [Inhabited α] : S α → α
+  subset : {α : Type u} → S α → S α → Prop := -- Cedar's defn is Bool instead of Prop, same below
     fun s₁ s₂ => ∀ a, mem s₁ a → mem s₂ a
   union : {α : Type u} → S α → S α → S α
   inter : {α : Type u} → S α → S α → S α
@@ -26,11 +31,24 @@ class VSetLikeF (S : Type u → Type v)
     fun s₁ s₂ => union (sdiff s₁ s₂) (sdiff s₂ s₁)
   disjoint : {α : Type u} → S α → S α → Prop :=
     fun s₁ s₂ => ∀ a, ¬(mem (inter s₁ s₂) a)
-  filter {α : Type u} (s : S α) (pred : α → Bool) : S α
+  -- filter {α : Type u} (s : S α) (pred : α → Bool) : S α
+  filter : {α : Type u} → (s : S α) → (pred : α → Bool) → S α
   ofList : {α : Type u} → List α → (S α) :=
     fun l => l.foldl (fun a s => insert s a) empty
+  isEmpty : S α → Prop :=
+    fun s => s = empty
+  isSingleton : {α : Type u} → S α → Prop :=
+    fun s => ∃ a, s = singleton a
+  findUniqueMinimal {α : Type u} [Inhabited α] : (S α) → (r : α → α → Bool) → α
+  findUniqueMaximal {α : Type u} [Inhabited α] : (S α) → (r : α → α → Bool) → α
+  all : {α : Type u} → (S α) → (α → Bool) → Prop :=
+    fun s p => ∀ a, mem s a → p a
+  any : {α : Type u} → (S α) → (α → Bool) → Prop :=
+    fun s p => ∃ a, mem s a ∧ p a
+  filterMap : {α β : Type u} → (α → Option β) → (S α) → S β
+  setIntRange : {α : Type u} → (a b : Int) → S α
 
-export VSetLikeF (symmDiff disjoint filter ofList)
+-- export VSetLikeF (symmDiff disjoint filter ofList)
 
 namespace VSetLikeF
 
@@ -80,6 +98,7 @@ class VSetInfF (S : Type u → Type v)
     fun s => card s ≠ none
   toList : {α : Type u} → (s : S α) → (h_finite : isFinite s) → List α
   fold {α : Type u} {β : Type u} (f : β → α → β) (init : β) : (s : S α) → (h_finite : isFinite s) → β
+  isFull : S α → Prop := fun s => s = full
 
 open VSetLikeF in
 class LawfulVSetLikeF (S : Type u → Type v) [VSetLikeF S]
@@ -91,7 +110,8 @@ class LawfulVSetLikeF (S : Type u → Type v) [VSetLikeF S]
   mem_insert_iff {a b : α} {s : S α} : b ∈ (s + a) ↔ b = a ∨ b ∈ s
   mem_remove_iff {a b : α} {s : S α} : b ∈ (s - a) ↔ b ≠ a ∧ b ∈ s
   mem_singleton_iff {a b : α} : b ∈ ({a} : S α) ↔ b = a
-  choose_mem {α : Type u} [Inhabited α] : ∀ (s : S α) (h : ∃ x, x ∈ s), choose s h ∈ s
+  -- choose_mem {α : Type u} [Inhabited α] : ∀ (s : S α) (h : ∃ x, x ∈ s), choose s h ∈ s
+  choose_mem {α : Type u} [Inhabited α] : ∀ (s : S α), (h : ∃ x, x ∈ s) → choose s ∈ s
   subset_iff {s₁ s₂ : S α} : s₁ ⊆ s₂ ↔ ∀ a, a ∈ s₁ → a ∈ s₂
   mem_union_iff  {a : α} {s₁ s₂ : S α} : a ∈ s₁ ∪ s₂ ↔ a ∈ s₁ ∨ a ∈ s₂
   mem_inter_iff  {a : α} {s₁ s₂ : S α} : a ∈ s₁ ∩ s₂ ↔ a ∈ s₁ ∧ a ∈ s₂
@@ -102,13 +122,12 @@ class LawfulVSetLikeF (S : Type u → Type v) [VSetLikeF S]
   mem_ofList_iff {a : α} {l : List α} : a ∈ (ofList l : S α) ↔ a ∈ l
   mem_map_iff {f : α → β} {s : S α} {b : β}
     : b ∈ f <$> s ↔ ∃ a, a ∈ s ∧ f a = b
+  mem_filterMap_iff {α β : Type u} {f : α → Option β} {s : S α} {b : β}
+    : b ∈ filterMap f s ↔ ∃ a, a ∈ s ∧ f a = some b
 
 open LawfulVSetLikeF in
 attribute [simp] not_mem_empty mem_singleton_iff mem_ofList_iff
 attribute [ext] LawfulVSetLikeF.ext
-
-class FoldCommutative (op : α → β → α) : Prop where
-  comm : (a : α) → (b₁ b₂ : β) → op (op a b₁) b₂ = op (op a b₂) b₁
 
 open VSetLikeF VSetF in
 class LawfulVSetF (S : Type u → Type v) [VSetF S]
@@ -129,25 +148,47 @@ attribute [simp] card_empty fold_empty
 open Std in
 def SetVstdTranslationNames : HashMap Lean.Name Lean.Name := HashMap.ofList <|
   List.map (f := fun ⟨x, y⟩ => (String.toName s!"Vstd.Set.{x}", String.toName y)) <| [
+  /- from current set.rs -/
+  -- Verus has no entry for `singleton`
+  ("empty", "VSetLikeF.empty"), -- or do we translate them to VSetF, by default assuming finite sets?
+  ("new", "VSetInfF.new"),
+  ("full", "VSetInfF.full"), -- might be an infinite set
   ("contains", "VSetLikeF.mem"),
   ("spec_has", "VSetLikeF.mem"),
-  ("empty", "VSetLikeF.empty"),
-  -- missing entry for `new`
-  ("insert", "VSetLikeF.insert"),
-  ("remove", "VSetLikeF.remove"),
-  -- no entry for singleton
-  ("choose", "VSetLikeF.choose"), -- The signatures for choose don't match
   ("subset_of", "VSetLikeF.subset"),
   ("spec_le", "VSetLikeF.subset"),
+  ("insert", "VSetLikeF.insert"),
+  ("remove", "VSetLikeF.remove"),
   ("union", "VSetLikeF.union"),
   ("spec_add", "VSetLikeF.union"),
   ("intersect", "VSetLikeF.inter"),
   ("spec_mul", "VSetLikeF.inter"),
   ("difference", "VSetLikeF.sdiff"),
   ("spec_sub", "VSetLikeF.sdiff"),
+  ("complement", "VSetInfF.compl"), -- might become an infinite set when taking complement
   ("filter", "VSetLikeF.filter"),
-  ("disjoint", "VSetLikeF.disjoint")
-  -- missing entries for `finite`, `len`, `complement`, etc.
+  ("finite", "VSetInfF.isFinite"), -- should be a property of the generic VSetLikeF instead
+  ("len", "VSetF.card"), -- assuming finiteness
+  -- CZ: the signature now matches, if we don't require a hypothesis that the set is inhabited
+  ("choose", "VSetLikeF.choose"), -- The signatures for choose don't match
+  ("mk_map", ""), -- ignored for now as Lean doesn't support build cycle, see Map/Defs.lean
+  ("disjoint", "VSetLikeF.disjoint"),
+
+  /- from current set_lib.rs -/
+  ("is_full", "VSetInfF.isFull"),
+  ("is_empty", "VSetLikeF.isEmpty"),
+  ("map", "Functor.map"),
+  ("to_seq", ""),
+  ("to_sorted_seq", ""),
+  ("is_singleton", "VSetLikeF.isSingleton"),
+  ("find_unique_minimal", "VSetLikeF.findUniqueMinimal"),
+  ("find_unique_maximal", "VSetLikeF.findUniqueMaximal"),
+  ("to_multiset", ""), -- ignored for now
+  ("all", "VSetLikeF.all"),
+  ("any", "VSetLikeF.any"),
+  ("filter_map", "VSetLikeF.filterMap"),
+  ("flatten", ""), -- ignored for now, as its type is different
+  ("set_int_range", "VSetLikeF.setIntRange"), -- if a set contains ints in [a,b), its size is bounded by b-a
 ]
 
 end Vstd
