VerusLean/Vstd/Map.lean
@@ -1,3 +1,3 @@
 import VerusLean.Vstd.Map.Basic
 import VerusLean.Vstd.Map.Defs
--- import VerusLean.Vstd.Map.Shim
+import VerusLean.Vstd.Map.Shim
