VerusLean/Vstd/Map/Basic.lean
@@ -1,17 +1,88 @@
+import VerusLean.Vstd.Set.Defs
 import VerusLean.Vstd.Map.Defs
 
 namespace Vstd
 
 namespace VMapLikeF
 
-variable {M : Type u → Type v → Type w} [VMapLikeF M] [LawfulVMapLikeF M] {α : Type u} {β : Type v}
+/-! # lawful maps -/
+open LawfulVMapLikeF
+
+variable {M : Type u → Type v → Type w}
+variable {S_key : Type u → Type w_key} [VSetLikeF S_key] [LawfulVSetLikeF S_key]
+variable {S_val : Type v → Type w_val} [VSetLikeF S_val] [LawfulVSetLikeF S_val]
+variable [LawfulVMapLikeF M S_key S_val]
+
+variable {α : Type u} {β : Type v} [DecidableEq α]
+
+-- CZ: If M is a lawful map, can we show that its domain is a lawful set?
+-- Maybe not - let's try write this as a definition
+
+omit [DecidableEq α]  in
+theorem map_empty : keys (∅ : M α β) = ∅ := by
+  simp
+
+theorem map_insert_domain (m : M α β) (key : α) (value : β):
+  keys (insert m key value) = VSetLikeF.insert key (keys m) := by
+  apply LawfulVSetLikeF.ext
+  intro x
+  by_cases h : x = key
+  . simp [h]
+    simp only [←memKeys_iff, memKeys_insert]
+  . simp [LawfulVSetLikeF.mem_insert_iff, h]
+    rw [memKeys_insert_iff]
+    simp [h]
+    exact value -- why do we need to show that `keys m` is inhabited?
+
+theorem map_insert_same (m : M α β) (key : α) (value : β):
+  get? (insert m key value) key = some value := by
+  simp [get?_insert]
+
+theorem map_insert_different (m : M α β) (key₁ key₂: α) (value : β) (h : key₁ ≠ key₂):
+  get? (insert m key₂ value) key₁ = get? m key₁ := by
+  simp [get?_insert]
+  intro h'; rw [h'] at h
+  contradiction
+
+theorem map_remove_domain (m : M α β) (key : α):
+  keys (remove m key) = VSetLikeF.remove key (keys m) := by
+  apply LawfulVSetLikeF.ext
+  intro x
+  by_cases h : x = key
+  . simp [h, memKeys_remove_iff]
+  . simp [h, memKeys_remove_iff, LawfulVSetLikeF.mem_remove_iff]
+
+theorem map_remove_different (m : M α β) (key₁ key₂: α) (h : key₁ ≠ key₂):
+  get? (remove m key₂) key₁ = get? m key₁ := by
+  simp [get?_remove]
+  intro h'; rw [h'] at h
+  contradiction
+
+theorem map_ext_equal (m₁ m₂ : M α β) :
+  (∀ (k : α), k ∈ keys m₁ ↔ k ∈ keys m₂ ∧ get? m₁ k = get? m₂ k) → m₁ = m₂ := by
+  apply LawfulVMapLikeF.ext
 
 @[simp]
 theorem insert_insert (m : M α β) (k : α) (v₁ v₂ : β) :
     insert (insert m k v₁) k v₂ = insert m k v₂ := by
-  ext
-  stop
-  done
+  apply LawfulVMapLikeF.ext
+  intro x
+  by_cases h : x = k
+  . simp only [h, memKeys_insert_iff]
+    simp [get?_insert, ←memKeys_iff, memKeys_insert]
+  . rw [get?_insert]
+    have h' : ¬k = x := by
+      intro p; have p' := p.symm; contradiction
+    simp [h', get?_insert]
+    rw [memKeys_insert_iff]
+    . simp [h]
+      rw [memKeys_insert_iff]
+      . simp [h]
+        rw [memKeys_insert_iff]
+        . simp [h]
+        . exact v₁
+      . exact v₁
+    . exact v₁
 
 end VMapLikeF /- namespace -/
 
