VerusLean/Vstd/Map/Shim.lean
@@ -1,11 +1,68 @@
+import VerusLean.Vstd.Set.Shim
 import VerusLean.Vstd.Map.Defs
 
 namespace Vstd
 
 inductive Map (α : Type u) (β : Type v)
-  | mk (elems : List α)
+  | mk (elems : List (α × β))
+deriving Repr, DecidableEq, Inhabited
 
-instance : VMapLikeF Map := by sorry
-instance : VMapF Map := by sorry
+instance M : VMapLikeF Map Set Set where
+  empty := .mk []
+  total := fun _ => .mk [] -- incorrect
+  new := fun _ _ => .mk [] -- incorrect
+  keys := fun m => match m with | .mk elems => S.ofList (elems.map Prod.fst)
+  values := fun m => match m with | .mk elems => S.ofList (elems.map Prod.snd)
+  get := fun m k h => match m with
+  | .mk elems =>
+    let entry := elems.find? (fun (k', _) => k' = k)
+    match entry with
+    | some (_, v) => v
+    | none => default -- should not occur given h
+  get? := fun m k =>
+    match m with
+    | .mk elems =>
+      let entry := elems.find? (fun (k', _) => k' = k)
+      entry.map Prod.snd
+  get! := fun m k =>
+    match m with
+    | .mk elems =>
+      let entry := elems.find? (fun (k', _) => k' = k)
+      match entry with
+      | some (_, v) => v
+      | none => default
+  insert := fun m k v => m -- incorrect
+  remove := fun m k => m -- incorrect
+  removeKeys := fun m ks => m -- incorrect
+  restrict := fun m ks => m -- incorrect
+  isEqualOnKey := fun m₁ m₂ k => match m₁, m₂ with
+    | .mk elems₁, .mk elems₂ =>
+      match elems₁.find? (fun (k', _) => k' = k), elems₂.find? (fun (k', _) => k' = k) with
+      | some (_, v₁), some (_, v₂) => v₁ = v₂
+      | _, _ => false
+  agrees := fun m₁ m₂ => match m₁, m₂ with
+    | .mk elems₁, .mk elems₂ =>
+      elems₁.all (fun (k₁, v₁) => match elems₂.find? (fun (k₂, _) => k₂ = k₁) with
+        | some (_, v₂) => v₁ = v₂
+        | none => false)
+  size := fun m => match m with | .mk elems => elems.length
+  submapOf := fun m₁ m₂ => match m₁, m₂ with
+    | .mk elems₁, .mk elems₂ =>
+      elems₁.all (fun (k₁, v₁) => match elems₂.find? (fun (k₂, _) => k₂ = k₁) with
+        | some (_, v₂) => v₁ = v₂
+        | none => false)
+  union_prefer_right := fun m₁ m₂ => m₂ -- incorrect
+  mapEntires := fun m f => match m with
+    | .mk elems => .mk (elems.map (fun (k, v) => (k, f k v)))
+  mapValues := fun m f => match m with
+    | .mk elems => .mk (elems.map (fun (k, v) => (k, f v)))
+  isInjective := fun _ => true -- incorrect
+    -- fun m => match m with
+    -- | .mk elems =>
+    --   let values := elems.map Prod.snd
+    --   values.Nodup
+
+
+-- instance : VMapF Map := by sorry
 
 end Vstd
