VerusLean/Vstd/Set/Shim.lean
@@ -4,26 +4,61 @@ namespace Vstd
 
 inductive Set (α : Type u)
   | mk (elems : List α)
+deriving Repr, DecidableEq, Inhabited
 
-instance : VSetLikeF Set where
+instance S : VSetLikeF Set where
   map := fun f s => match s with | .mk elems => .mk (elems.map f)
-  mem := fun s a => match s with | .mk elems => a ∈ elems
+  -- mem := fun s a => match s with | .mk elems => a ∈ elems
+  -- Cedar requires [DecidableEq α]
+  -- mem := fun {α} [DecidableEq α] (s : Set α) (a : α) => match s with
+    -- | .mk elems => elems.contains a
+  mem := fun _ _ => false -- This is totally wrong
   empty := .mk []
+  -- no correspondence in Cedar
   insert := fun a s => match s with | .mk elems => .mk (a :: elems)
+  -- no correspondence in Cedar
   remove := fun _ s => match s with | .mk elems => .mk (elems)  -- This is incorrect
-  choose := fun _ _ => default  -- This is totally wrong
+  -- singleton := fun a => .mk [a]
+  -- no correspondence in Cedar
+  choose := fun s => match s with
+    | .mk elems => match elems with
+      | [] => default
+      | (x :: _) => x
+  subset := fun _ _ => false -- This is totally wrong
   union := fun s₁ s₂ => match s₁, s₂ with
     | .mk elems₁, .mk elems₂ => .mk (elems₁ ++ elems₂)
   inter := fun s₁ s₂ => match s₁, s₂ with
     | .mk elems₁, .mk _ => .mk (elems₁) -- This is incorrect
   sdiff := fun s₁ s₂ => match s₁, s₂ with
     | .mk elems₁, .mk _ => .mk (elems₁) -- This is incorrect
+  disjoint := fun _ _ => false -- This is incorrect
   filter := fun s p => match s with
     | .mk elems => .mk (elems.filter p)
+  findUniqueMinimal := fun _ _ => default -- This is incorrect
+  findUniqueMaximal := fun _ _ => default -- This is incorrect
+  all := fun s p => match s with
+    | .mk elems => elems.all p
+  any := fun s p => match s with
+    | .mk elems => elems.any p
+  filterMap := fun _ _ => .mk [] -- This is incorrect
+  setIntRange := fun _ _ => .mk [] -- This is incorrect
 
-instance : VSetF Set where
+instance FS : VSetF Set where
   card := fun s => match s with | .mk elems => elems.length
   toList := fun s => match s with | .mk elems => elems -- This is slightly incorrect
   fold := fun f init s => match s with | .mk elems => elems.foldl f init
+
+instance IS : VSetInfF Set where
+  full := .mk [] -- This is incorrect
+  new := fun _ => .mk [] -- This is incorrect
+  compl := fun s => match s with
+    | .mk elems => .mk [] -- This is incorrect
+  card := fun s => match s with
+    | .mk elems => some elems.length
+  toList := fun s h_finite => match s with
+    | .mk elems => elems -- how to use h_finite?
+  fold := fun f init s h_finite => match s with
+    | .mk elems => elems.foldl f init -- how to use h_finite?
+
 
 end Vstd
